@prefix rdf: <http://www.w3.org/1999/02/22-rdf-syntax-ns#> .
@prefix foaf: <http://xmlns.com/foaf/0.1/> .
@prefix dctype: <http://purl.org/dc/dcmitype/> .
@prefix dct: <http://purl.org/dc/terms/> .
@prefix dc: <http://purl.org/dc/elements/1.1/> .
@prefix rdfs: <http://www.w3.org/2000/01/rdf-schema#> .
@prefix owl: <http://www.w3.org/2002/07/owl#> .
@prefix xsd: <http://www.w3.org/2001/XMLSchema#> .
@prefix ns0: <http://iandavis.com/id/> .
@prefix skos: <http://www.w3.org/2004/02/skos/core#> .
@prefix ov: <http://open.vocab.org/terms/> .
@prefix ns1: <http://lists.foaf-project.org/mailman/listinfo/> .
@prefix vann: <http://purl.org/vocab/vann/> .
@prefix bio: <http://purl.org/vocab/bio/0.1/> .
@prefix msg0: <http://web.resource.org/cc/> .
@prefix ns2: <http://purl.org/NET/c4dm/event.owl#> .
@prefix cyc: <http://sw.opencyc.org/2009/04/07/concept/en/> .
@prefix ns3: <http://linkedevents.org/ontology/> .
@prefix status: <http://www.w3.org/2003/06/sw-vocab-status/ns#> .
@prefix mo: <http://purl.org/ontology/mo/> .
@prefix ns4: <http://www.w3.org/2006/time#> .
@prefix rel: <http://purl.org/vocab/relationship/> .
@prefix label: <http://purl.org/net/vocab/2004/03/label#> .

<http://vocab.org/bio/0.1/.turtle> rdf:type foaf:Document ,
                                            dctype:Text ;
                                   foaf:primaryTopic <http://purl.org/vocab/bio/0.1/> ;
                                   dct:hasFormat <http://vocab.org/bio/0.1/.rdf> ,
                                                 <http://vocab.org/bio/0.1/.html> ,
                                                 <http://vocab.org/bio/0.1/.json> ;
                                   foaf:topic <http://purl.org/vocab/bio/0.1/> .

<http://vocab.org/bio/0.1/.rdf> rdf:type dctype:Text ,
                                         foaf:Document ;
                                dc:format "application/rdf+xml" ;
                                rdfs:label "RDF/XML" .

<http://vocab.org/bio/0.1/.html> rdf:type dctype:Text ,
                                          foaf:Document ;
                                 dc:format "text/html" ;
                                 rdfs:label "HTML" .

<http://vocab.org/bio/0.1/.json> rdf:type dctype:Text ,
                                          foaf:Document ;
                                 dc:format "application/json" ;
                                 rdfs:label "JSON" .

<http://purl.org/vocab/bio/0.1/> rdf:type owl:Ontology ;
                                 dct:title "BIO: A vocabulary for biographical information"@en ;
                                 dct:date "2010-05-10"^^xsd:date ;
                                 dct:abstract "This document describes a vocabulary for describing biographical information about people, both living and dead. "@en ;
                                 dct:description """<div>
        
        <p>The BIO vocabulary contains terms useful for finding out more about people and their backgrounds and has some cross-over into genealogical information. 
        The approach taken is to describe a person's life as a series of interconnected key events, around which other information can be woven. 
        This vocabulary defines the event framework and supplies a set of core event types that cover many use cases, but it is expected that it 
        will be extended in other vocabularies to suit their needs. The intention of this vocabulary is to describe biographical events of people 
        and this intention carries through to the definitions of the properties and classes which are person-centric rather than neutral. For example 
        the Employment event puts the person being employed as the principal agent in the event rather than the employer.</p>
        <p>The BIO vocabulary defines a number of core classes and properties for describing biographical information: </p>
        <p><figure><img src="/bio/core-classes.png"></img><br></br>Figure: Biography Vocabulary Core Classes (<a href="http://vocab.org/bio/core-classes.png">PNG version</a>, <a href="http://vocab.org/bio/core-classes.svg">SVG version</a>)</figure></p>
        <p>At its heart the BIO vocabulary is concerned with people, their relationships and the events in their lives. Together these can be
        used to build up a narrative of a person's life and their interactions with other people, organizations and the world around them. Events bound intervals
        of time that may be associated with particular relationships between people and groups or organisations. Many different types of life event are
        defined in this vocabulary including the obvious Birth, Marriage and Death but also Coronation, Performance and even Murder. These events are not intended
        to be fully comprehensive but are representative of the types of events associated with biographical material. Currently the relationship segment of the
        vocabulary is underspecified with only a generic Relationship class available. It is envisaged that many types of relationship such as families, employments
        and ownerships will be specified in the future.</p>
        <p>The sequence of events and intervals build a timeline of history against which people and their relationships can be placed. The aim is
        to enable simple forms of genealogical reasoning such as determining whether a child was born out of wedlock or the location of a family
        given the fact one of their children was attending a particular school. Events are ordered in time by relating them to one another and to abstract
        intervals of time:</p>
        <p><figure><img src="/bio/timelines.png"></img><br></br>Figure: Biography Vocabulary Timelines(<a href="http://vocab.org/bio/timelines.png">PNG version</a>, <a href="http://vocab.org/bio/timelines.svg">SVG version</a>)</figure></p>
        <p>Please see <a href="https://github.com/iand/vocab-bio">https://github.com/iand/vocab-bio</a> for the master version of this vocabulary.</p>
      </div>"""^^rdf:XMLLiteral ;
                                 dct:identifier "http://purl.org/vocab/bio/0.1/schema" ;
                                 dct:creator ns0:me ,
                                             "David Galbraith" ;
                                 dct:rights "Copyright © 2002-2010 Ian Davis and David Galbraith" ;
                                 dct:issued "2003-03-07"^^xsd:date ;
                                 skos:historyNote _:mor54413383902b4 ,
                                                  _:mor544133839048c ,
                                                  _:mor54413383905a0 ,
                                                  _:mor54413383905fb ,
                                                  _:mor5441338390656 ,
                                                  _:mor54413383906b2 ,
                                                  _:mor544133839070f ,
                                                  _:mor5441338390769 ;
                                 skos:changeNote _:mor544133839031d ,
                                                 _:mor5441338390378 ,
                                                 _:mor54413383903d6 ,
                                                 _:mor544133839042f ,
                                                 _:mor54413383904ec ,
                                                 _:mor5441338390548 ;
                                 ov:discussionList ns1:foaf-dev ;
                                 vann:preferredNamespaceUri "http://purl.org/vocab/bio/0.1/" ;
                                 vann:preferredNamespacePrefix "bio" ;
                                 vann:example <http://purl.org/vocab/bio/examples/1> ;
                                 vann:termGroup bio:termgroup1 ,
                                                bio:termgroup2 ,
                                                bio:termgroup3 ,
                                                bio:termgroup4 ,
                                                bio:termgroup5 .

ns0:me rdf:type foaf:Person ;
       foaf:name "Ian Davis" .

_:mor54413383902b4 rdf:value "Added keywords property" ;
                   dct:date "2003-07-28" ;
                   dct:creator "Ian Davis" .

_:mor544133839031d rdf:value "Added Creative Commons license" ;
                   dct:date "2004-03-05" ;
                   dct:creator "Ian Davis" .

_:mor5441338390378 rdf:value "Added examples" ;
                   dct:date "2005-04-01" ;
                   dct:creator "Ian Davis" .

_:mor54413383903d6 rdf:value "Minor changes to improve publishing process" ;
                   dct:date "2009-05-19" ;
                   dct:creator "Ian Davis" .

_:mor544133839042f rdf:value "Added change history" ;
                   dct:date "2010-04-20" ;
                   dct:creator "Ian Davis" .

_:mor544133839048c rdf:value "Major expansion of properties and classes" ;
                   dct:date "2010-05-10" ;
                   dct:creator "Ian Davis" .

_:mor54413383904ec rdf:value "Batch of revisions based on community feedback" ;
                   dct:date "2010-05-20" ;
                   dct:creator "Ian Davis" .

_:mor5441338390548 rdf:value "Expanded description and added diagrams" ;
                   dct:date "2011-06-14" ;
                   dct:creator "Ian Davis" .

_:mor54413383905a0 rdf:value "Added biography property" ;
                   dct:date "2010-06-05" ;
                   dct:creator "Ian Davis" .

_:mor54413383905fb rdf:value "Added subproperty and equivalent property relations for bio:father, bio:mother and bio:child" ;
                   dct:date "2010-06-06" ;
                   dct:creator "Ian Davis" .

_:mor5441338390656 rdf:value "Added bio:Formation and bio:Disbanding events" ;
                   dct:date "2011-06-10" ;
                   dct:creator "Ian Davis" .

_:mor54413383906b2 rdf:value "Added bio:Performance event" ;
                   dct:date "2011-06-10" ;
                   dct:creator "Ian Davis" .

_:mor544133839070f rdf:value "Added bio:Relationship class and properties" ;
                   dct:date "2011-06-14" ;
                   dct:creator "Ian Davis" .

_:mor5441338390769 rdf:value "Added properties for Birth and Death Event types, motivated by JSON serialisations of RDF" ;
                   dct:date "2011-06-14" ;
                   dct:creator "Alexandre Passant" .

ns1:foaf-dev rdfs:label "FOAF-DEV mailing list" .

<file:///var/www/vocab.org/www/htdocs/bio/> rdf:type msg0:Work ;
                                            msg0:license <http://creativecommons.org/licenses/by/1.0/> ;
                                            dct:type dctype:Text .

<http://creativecommons.org/licenses/by/1.0/> rdf:type msg0:License ;
                                              msg0:permits msg0:Reproduction ,
                                                           msg0:Distribution ,
                                                           msg0:DerivativeWorks ;
                                              msg0:requires msg0:Notice ,
                                                            msg0:Attribution .

foaf:Person rdf:type owl:Class ;
            owl:equivalentClass _:mor5441338390826 .

_:mor5441338390826 rdf:type owl:Class ;
                   owl:intersectionOf _:mor5441338390873 .

_:mor5441338390873 rdf:first _:mor54413383908b6 ;
                   rdf:rest _:mor5441338390913 .

_:mor54413383908b6 rdf:type owl:Restriction ;
                   owl:cardinality "1"^^xsd:nonNegativeInteger ;
                   owl:onProperty bio:father .

_:mor5441338390913 rdf:first _:mor5441338390956 ;
                   rdf:rest rdf:nil .

_:mor5441338390956 rdf:type owl:Restriction ;
                   owl:cardinality "1"^^xsd:nonNegativeInteger ;
                   owl:onProperty bio:mother .

bio:Event rdf:type owl:Class ;
          rdfs:label "Event"@en ;
          rdfs:comment "An event is an occurrence that brings about a change in the state of affairs for one or more people and/or other agents. Events are assumed to occur over a period of time and may not have precise start and end points."@en ;
          vann:usageNote "This class is intended to describe biographical events, i.e. events in the life of a person."@en ;
          rdfs:isDefinedBy <http://purl.org/vocab/bio/0.1/> ;
          rdfs:subClassOf ns2:Event ,
                          cyc:Event ,
                          ns3:Event ,
                          dctype:Event ;
          skos:historyNote _:mor54413383909eb ,
                           _:mor5441338390aff ;
          status:term_status "testing" ;
          skos:changeNote _:mor5441338390a4a ,
                          _:mor5441338390aa4 .

_:mor54413383909eb rdf:value "Made equivalent to cyc:Event" ;
                   dct:date "2010-05-04" ;
                   dct:creator "Ian Davis" .

_:mor5441338390a4a rdf:value "Marked as a stable term" ;
                   dct:date "2010-05-04" ;
                   dct:creator "Ian Davis" .

_:mor5441338390aa4 rdf:value "Marked as testing status" ;
                   dct:date "2010-05-20" ;
                   dct:creator "Ian Davis" .

_:mor5441338390aff rdf:value "Removed subclass of owl-time ProperInteval" ;
                   dct:date "2010-05-20" ;
                   dct:creator "Ian Davis" .

bio:IndividualEvent rdf:type owl:Class ;
                    rdfs:label "Individual Event"@en ;
                    rdfs:comment "A type of event that is principally about a single person, group or organization. Other agents may be involved but the event is most significant for the principal agent."@en ;
                    rdfs:subClassOf bio:Event ,
                                    _:mor5441338390b78 ;
                    rdfs:isDefinedBy <http://purl.org/vocab/bio/0.1/> ;
                    status:term_status "unstable" .

_:mor5441338390b78 rdf:type owl:Restriction ;
                   owl:cardinality "1"^^xsd:nonNegativeInteger ;
                   owl:onProperty bio:principal .

bio:GroupEvent rdf:type owl:Class ;
               rdfs:label "Group Event"@en ;
               rdfs:comment "A type of event that is principally about one or more agents and their partnership. Other agents may be involved but the event is most significant for the partner agent."@en ;
               rdfs:subClassOf bio:Event ,
                               _:mor5441338390bfa ;
               rdfs:isDefinedBy <http://purl.org/vocab/bio/0.1/> ;
               status:term_status "unstable" .

_:mor5441338390bfa rdf:type owl:Restriction ;
                   owl:minCardinality "2"^^xsd:nonNegativeInteger ;
                   owl:onProperty bio:partner .

bio:Birth rdf:type owl:Class ;
          rdfs:label "Birth"@en ;
          rdfs:comment "The event of a person entering into life."@en ;
          rdfs:subClassOf bio:IndividualEvent ;
          rdfs:isDefinedBy <http://purl.org/vocab/bio/0.1/> ;
          status:term_status "testing" ;
          skos:changeNote _:mor5441338390c79 ;
          vann:example _:mor5441338390cd3 .

_:mor5441338390c79 rdf:value "Marked as testing" ;
                   dct:date "2010-05-04" ;
                   dct:creator "Ian Davis" .

_:mor5441338390cd3 rdf:type ov:SchemaExample ;
                   rdfs:label "The birth of Albert Einstein" ;
                   rdfs:comment '''
        <pre><code>_:e a bio:Birth 
    ; dc:date "1879-03-14"
    ; bio:principal &lt;http://dbpedia.org/resource/Albert_Einstein&gt;
    ; bio:parent &lt;http://dbpedia.org/resource/Pauline_Koch&gt;
    ; bio:parent &lt;http://dbpedia.org/resource/Hermann_Einstein&gt;
    ; bio:place &lt;http://dbpedia.org/resource/Ulm&gt;
    .</code></pre>
'''^^rdf:XMLLiteral .

bio:Marriage rdf:type owl:Class ;
             rdfs:label "Marriage"@en ;
             rdfs:comment "The event of creating uniting the participants into a new family unit, sometimes accompanied by a formal wedding ceremony. This is intended to cover a broad range of marriages including those given formal legal standing, common-law, or by convention. It is not restricted to marriages of two people of the opposite gender, but also includes polygamous and same-sex unions."@en ;
             rdfs:subClassOf bio:GroupEvent ;
             rdfs:isDefinedBy <http://purl.org/vocab/bio/0.1/> ;
             status:term_status "stable" ;
             skos:changeNote _:mor5441338390d54 ;
             owl:equivalentClass cyc:WeddingEvent_Generic ;
             skos:historyNote _:mor5441338390db3 ;
             vann:example _:mor5441338390e0c .

_:mor5441338390d54 rdf:value "Marked as a stable term" ;
                   dct:date "2010-05-04" ;
                   dct:creator "Ian Davis" .

_:mor5441338390db3 rdf:value "Made equivalent to cyc:WeddingEvent_Generic" ;
                   dct:date "2010-05-04" ;
                   dct:creator "Ian Davis" .

_:mor5441338390e0c rdf:type ov:SchemaExample ;
                   rdfs:label "The marriage of Albert Einstein and Mileva Marić" ;
                   rdfs:comment '''
        <pre><code>_:e a bio:Marriage 
    ; dc:date "1903"
    ; bio:partner &lt;http://dbpedia.org/resource/Albert_Einstein&gt;
    ; bio:partner &lt;http://dbpedia.org/resource/Mileva_Mari%C4%87&gt;
    ; bio:place &lt;http://dbpedia.org/resource/Bern&gt;
    .</code></pre>
'''^^rdf:XMLLiteral .

bio:Death rdf:type owl:Class ;
          rdfs:label "Death"@en ;
          rdfs:comment "The event of a person's life ending."@en ;
          rdfs:subClassOf bio:IndividualEvent ;
          rdfs:isDefinedBy <http://purl.org/vocab/bio/0.1/> ;
          status:term_status "stable" ;
          skos:changeNote _:mor5441338390e86 ;
          vann:example _:mor5441338390ee2 .

_:mor5441338390e86 rdf:value "Marked as a stable term" ;
                   dct:date "2010-05-04" ;
                   dct:creator "Ian Davis" .

_:mor5441338390ee2 rdf:type ov:SchemaExample ;
                   rdfs:label "The death of Albert Einstein" ;
                   rdfs:comment '''
        <pre><code>_:e a bio:Death 
    ; dc:date "1955-04-18"
    ; bio:principal &lt;http://dbpedia.org/resource/Albert_Einstein&gt;
    ; bio:place &lt;http://dbpedia.org/resource/Princeton,_New_Jersey&gt;
    .</code></pre>
'''^^rdf:XMLLiteral .

bio:Annulment rdf:type owl:Class ;
              rdfs:label "Annulment"@en ;
              rdfs:comment "The event of declaring a marriage void from the beginning as though it never existed."@en ;
              rdfs:subClassOf bio:GroupEvent ;
              rdfs:isDefinedBy <http://purl.org/vocab/bio/0.1/> ;
              status:term_status "unstable" ;
              dct:issued "2010-05-03" .

bio:Divorce rdf:type owl:Class ;
            rdfs:label "Divorce"@en ;
            rdfs:comment "The event of legally dissolving a marriage."@en ;
            rdfs:subClassOf bio:GroupEvent ;
            rdfs:isDefinedBy <http://purl.org/vocab/bio/0.1/> ;
            status:term_status "unstable" ;
            dct:issued "2010-05-03" ;
            vann:example _:mor5441338390f6e .

_:mor5441338390f6e rdf:type ov:SchemaExample ;
                   rdfs:label "The divorce of Albert Einstein and Mileva Marić" ;
                   rdfs:comment '''
        <pre><code>_:e a bio:Divorce 
    ; dc:date "1919-02-14"
    ; bio:partner &lt;http://dbpedia.org/resource/Albert_Einstein&gt;
    ; bio:partner &lt;http://dbpedia.org/resource/Mileva_Mari%C4%87&gt;
    ; bio:place &lt;http://dbpedia.org/resource/Zurich&gt;
    .</code></pre>
'''^^rdf:XMLLiteral .

bio:Funeral rdf:type owl:Class ;
            rdfs:label "Funeral"@en ;
            rdfs:comment "The event of marking a person's death with a ceremony."@en ;
            rdfs:subClassOf bio:IndividualEvent ;
            rdfs:isDefinedBy <http://purl.org/vocab/bio/0.1/> ;
            status:term_status "unstable" ;
            dct:issued "2010-05-03" .

bio:Burial rdf:type owl:Class ;
           rdfs:label "Burial"@en ;
           rdfs:comment "The event of interring the remains of a person's body into the ground."@en ;
           rdfs:subClassOf bio:IndividualEvent ;
           rdfs:isDefinedBy <http://purl.org/vocab/bio/0.1/> ;
           status:term_status "unstable" ;
           dct:issued "2010-05-03" .

bio:Cremation rdf:type owl:Class ;
              rdfs:label "Cremation"@en ;
              rdfs:comment "The event of disposing of the remains of a person's body by fire."@en ;
              rdfs:subClassOf bio:IndividualEvent ;
              rdfs:isDefinedBy <http://purl.org/vocab/bio/0.1/> ;
              status:term_status "unstable" ;
              dct:issued "2010-05-03" ;
              vann:example _:mor544133839100f .

_:mor544133839100f rdf:type ov:SchemaExample ;
                   rdfs:label "The cremation of Albert Einstein" ;
                   rdfs:comment '''
        <pre><code>_:e a bio:Cremation 
    ; dc:date "1955-04-18"
    ; bio:principal &lt;http://dbpedia.org/resource/Albert_Einstein&gt;
    ; bio:place &lt;http://dbpedia.org/resource/Princeton,_New_Jersey&gt;
    .</code></pre>
'''^^rdf:XMLLiteral .

bio:Adoption rdf:type owl:Class ;
             rdfs:label "Adoption"@en ;
             rdfs:comment "The event of creating of a legal parent/child relationship that does not exist biologically."@en ;
             rdfs:subClassOf bio:IndividualEvent ;
             rdfs:isDefinedBy <http://purl.org/vocab/bio/0.1/> ;
             status:term_status "unstable" ;
             dct:issued "2010-05-03" .

bio:Baptism rdf:type owl:Class ;
            rdfs:label "Baptism"@en ;
            rdfs:comment "The ceremonial event held to admit a person to membership of a Christian church."@en ;
            rdfs:subClassOf bio:IndividualEvent ;
            rdfs:isDefinedBy <http://purl.org/vocab/bio/0.1/> ;
            status:term_status "unstable" ;
            skos:changeNote _:mor54413383910a0 ;
            dct:issued "2010-05-03" .

_:mor54413383910a0 rdf:value "Revised comment, replacing 'the Christian church' with 'a Christian church' " ;
                   dct:date "2010-05-20" ;
                   dct:creator "Ian Davis" .

bio:BarMitzvah rdf:type owl:Class ;
               rdfs:label "BarMitzvah"@en ;
               rdfs:comment "The ceremonial event held when a Jewish boy reaches age 13."@en ;
               rdfs:subClassOf bio:IndividualEvent ;
               rdfs:isDefinedBy <http://purl.org/vocab/bio/0.1/> ;
               status:term_status "unstable" ;
               dct:issued "2010-05-03" .

bio:BasMitzvah rdf:type owl:Class ;
               rdfs:label "BasMitzvah"@en ;
               rdfs:comment 'The ceremonial event held when a Jewish girl reaching age 13, also known as "Bat Mitzvah."'@en ;
               rdfs:subClassOf bio:IndividualEvent ;
               rdfs:isDefinedBy <http://purl.org/vocab/bio/0.1/> ;
               status:term_status "unstable" ;
               dct:issued "2010-05-03" .

bio:Execution rdf:type owl:Class ;
              rdfs:label "Execution"@en ;
              rdfs:comment "The event of a person being deliberately killed as punishment."@en ;
              rdfs:subClassOf bio:Death ;
              rdfs:isDefinedBy <http://purl.org/vocab/bio/0.1/> ;
              status:term_status "unstable" ;
              dct:issued "2010-05-05" .

bio:Assassination rdf:type owl:Class ;
                  rdfs:label "Assassination"@en ;
                  rdfs:comment "The event of a person being deliberately targeted and killed."@en ;
                  rdfs:subClassOf bio:Murder ;
                  rdfs:isDefinedBy <http://purl.org/vocab/bio/0.1/> ;
                  status:term_status "unstable" ;
                  dct:issued "2010-05-05" .

bio:Murder rdf:type owl:Class ;
           rdfs:label "Murder"@en ;
           rdfs:comment "The event of a person being killed unlawfully with intent by the killer."@en ;
           rdfs:subClassOf bio:Death ;
           rdfs:isDefinedBy <http://purl.org/vocab/bio/0.1/> ;
           status:term_status "unstable" ;
           dct:issued "2010-05-05" .

bio:Ordination rdf:type owl:Class ;
               rdfs:label "Ordination"@en ;
               rdfs:comment "The ceremonial event held when a person receives authority to act in religious matters."@en ;
               rdfs:subClassOf bio:IndividualEvent ;
               rdfs:isDefinedBy <http://purl.org/vocab/bio/0.1/> ;
               status:term_status "unstable" ;
               dct:issued "2010-05-03" .

bio:Naturalization rdf:type owl:Class ;
                   rdfs:label "Naturalization"@en ;
                   rdfs:comment "The event of a person obtaining citizenship. Note that the place the naturalization event occurs at may be different from the state the person is obtaining citizenship of. "@en ;
                   rdfs:subClassOf bio:IndividualEvent ;
                   rdfs:isDefinedBy <http://purl.org/vocab/bio/0.1/> ;
                   status:term_status "unstable" ;
                   dct:issued "2010-05-03" ;
                   vann:example _:mor544133839118a .

_:mor544133839118a rdf:type ov:SchemaExample ;
                   rdfs:label "Albert Einstein becoming a citizen of the United States" ;
                   rdfs:comment '''
        <pre><code>_:e a bio:Emigration 
    ; dc:date "1940"
    ; bio:principal &lt;http://dbpedia.org/resource/Albert_Einstein&gt;
    ; bio:state &lt;http://dbpedia.org/resource/United_States&gt;
    .</code></pre>
'''^^rdf:XMLLiteral .

bio:Emigration rdf:type owl:Class ;
               rdfs:label "Emigration"@en ;
               rdfs:comment "The event of a person leaving their homeland with the intent of residing elsewhere."@en ;
               rdfs:subClassOf bio:IndividualEvent ;
               rdfs:isDefinedBy <http://purl.org/vocab/bio/0.1/> ;
               status:term_status "unstable" ;
               dct:issued "2010-05-03" ;
               vann:example _:mor544133839120b .

_:mor544133839120b rdf:type ov:SchemaExample ;
                   rdfs:label "Albert Einstein emigrating to the United States" ;
                   rdfs:comment '''
        <pre><code>_:e a bio:Emigration 
    ; dc:date "1933"^^xsd:gYear
    ; bio:principal &lt;http://dbpedia.org/resource/Albert_Einstein&gt;
    ; bio:state &lt;http://dbpedia.org/resource/United_States&gt;
    .</code></pre>
'''^^rdf:XMLLiteral .

bio:Enrolment rdf:type owl:Class ;
              rdfs:label "Enrolment"@en ;
              rdfs:comment "The event of a person initiating attendence to a school or other place of learning."@en ;
              rdfs:subClassOf bio:IndividualEvent ;
              rdfs:isDefinedBy <http://purl.org/vocab/bio/0.1/> ;
              status:term_status "unstable" ;
              dct:issued "2010-05-03" .

bio:Graduation rdf:type owl:Class ;
               rdfs:label "Graduation"@en ;
               rdfs:comment "The event of a person being awarded educational diplomas or degrees."@en ;
               rdfs:subClassOf bio:IndividualEvent ;
               rdfs:isDefinedBy <http://purl.org/vocab/bio/0.1/> ;
               status:term_status "unstable" ;
               dct:issued "2010-05-03" ;
               vann:example _:mor544133839129d .

_:mor544133839129d rdf:type ov:SchemaExample ;
                   rdfs:label "Albert Einstein receiving his Doctorate from the University of Zurich" ;
                   rdfs:comment '''
        <pre><code>_:e a bio:Graduation 
    ; dc:date "1905"^^xsd:gYear
    ; bio:principal &lt;http://dbpedia.org/resource/Albert_Einstein&gt;
    ; bio:organization &lt;http://dbpedia.org/resource/University_of_Zurich&gt;
    .</code></pre>
'''^^rdf:XMLLiteral .

bio:Imprisonment rdf:type owl:Class ;
                 rdfs:label "Imprisonment"@en ;
                 rdfs:comment "The event of a person being detained in a jail or prison."@en ;
                 rdfs:subClassOf bio:IndividualEvent ;
                 rdfs:isDefinedBy <http://purl.org/vocab/bio/0.1/> ;
                 status:term_status "unstable" ;
                 dct:issued "2010-05-04" .

bio:Employment rdf:type owl:Class ;
               rdfs:label "Employment"@en ;
               rdfs:comment "The event of a person entering an occupational relationship with an employer."@en ;
               rdfs:subClassOf bio:IndividualEvent ;
               rdfs:isDefinedBy <http://purl.org/vocab/bio/0.1/> ;
               status:term_status "unstable" ;
               dct:issued "2010-05-03" .

bio:PositionChange rdf:type owl:Class ;
                   rdfs:label "Change of Position"@en ;
                   rdfs:comment "The event of a person changing the position they hold with an employer."@en ;
                   rdfs:subClassOf bio:IndividualEvent ;
                   rdfs:isDefinedBy <http://purl.org/vocab/bio/0.1/> ;
                   status:term_status "unstable" ;
                   dct:issued "2010-05-03" .

bio:NameChange rdf:type owl:Class ;
               rdfs:label "Change of Name"@en ;
               rdfs:comment "The event of a person changing their name."@en ;
               rdfs:subClassOf bio:IndividualEvent ;
               rdfs:isDefinedBy <http://purl.org/vocab/bio/0.1/> ;
               status:term_status "unstable" ;
               dct:issued "2010-05-03" .

bio:Promotion rdf:type owl:Class ;
              rdfs:label "Promotion"@en ;
              rdfs:comment "The event of a person changing the position they hold with an employer to one with more importance or responsibility."@en ;
              rdfs:subClassOf bio:PositionChange ;
              rdfs:isDefinedBy <http://purl.org/vocab/bio/0.1/> ;
              status:term_status "unstable" ;
              dct:issued "2010-05-03" .

bio:Demotion rdf:type owl:Class ;
             rdfs:label "Demotion"@en ;
             rdfs:comment "The event of a person changing the position they hold with an employer to one with less importance or responsibility."@en ;
             rdfs:subClassOf bio:PositionChange ;
             rdfs:isDefinedBy <http://purl.org/vocab/bio/0.1/> ;
             status:term_status "unstable" ;
             dct:issued "2010-05-03" .

bio:Retirement rdf:type owl:Class ;
               rdfs:label "Retirement"@en ;
               rdfs:comment "The event of a person exiting an occupational relationship with an employer after a qualifying time period. In many cultures retirement is expected and even required once the person reaches a particular age."@en ;
               rdfs:subClassOf bio:IndividualEvent ;
               rdfs:isDefinedBy <http://purl.org/vocab/bio/0.1/> ;
               status:term_status "unstable" ;
               dct:issued "2010-05-03" .

bio:Resignation rdf:type owl:Class ;
                rdfs:label "Resignation"@en ;
                rdfs:comment "The event of a person voluntarily giving up or quitting their office or position."@en ;
                rdfs:subClassOf bio:IndividualEvent ;
                rdfs:isDefinedBy <http://purl.org/vocab/bio/0.1/> ;
                status:term_status "unstable" ;
                dct:issued "2010-05-03" .

bio:Dismissal rdf:type owl:Class ;
              rdfs:label "Dismissal"@en ;
              rdfs:comment "The event of a person involuntarily giving up their office or position. Dismissal is often perceived to be the employee's fault and may be considered disgraceful."@en ;
              rdfs:subClassOf bio:IndividualEvent ;
              rdfs:isDefinedBy <http://purl.org/vocab/bio/0.1/> ;
              status:term_status "unstable" ;
              dct:issued "2010-05-03" .

bio:Redundancy rdf:type owl:Class ;
               rdfs:label "Redundancy"@en ;
               rdfs:comment "The event of a person involuntarily giving up an office or position that is no longer needed. Redundancy is usually perceived to be the employer's fault and is usually due to conditions outside of the employee's control."@en ;
               rdfs:subClassOf bio:IndividualEvent ;
               rdfs:isDefinedBy <http://purl.org/vocab/bio/0.1/> ;
               status:term_status "unstable" ;
               dct:issued "2010-05-03" .

bio:Investiture rdf:type owl:Class ;
                rdfs:label "Investiture"@en ;
                rdfs:comment "The ceremonial event of a person taking a public office or honour."@en ;
                rdfs:subClassOf bio:IndividualEvent ;
                rdfs:isDefinedBy <http://purl.org/vocab/bio/0.1/> ;
                status:term_status "unstable" ;
                dct:issued "2010-05-03" .

bio:Inauguration rdf:type owl:Class ;
                 rdfs:label "Inauguration"@en ;
                 rdfs:comment "The ceremonial event marking the beginning of a person's term of office as a leader."@en ;
                 rdfs:subClassOf bio:IndividualEvent ;
                 rdfs:isDefinedBy <http://purl.org/vocab/bio/0.1/> ;
                 status:term_status "unstable" ;
                 dct:issued "2010-05-03" .

bio:Accession rdf:type owl:Class ;
              rdfs:label "Accession"@en ;
              rdfs:comment "The event of a person succeeding to the right to hold regal power. This event is often automatic on the death of the previous monarch and is usually followed by a coronation event."@en ;
              rdfs:subClassOf bio:IndividualEvent ;
              rdfs:isDefinedBy <http://purl.org/vocab/bio/0.1/> ;
              status:term_status "unstable" ;
              dct:issued "2010-05-03" .

bio:Coronation rdf:type owl:Class ;
               rdfs:label "Coronation"@en ;
               rdfs:comment "The ceremonial event of a person being invested with regal power to become a monarch."@en ;
               rdfs:subClassOf bio:IndividualEvent ;
               rdfs:isDefinedBy <http://purl.org/vocab/bio/0.1/> ;
               status:term_status "unstable" ;
               dct:issued "2010-05-03" .

bio:Formation rdf:type owl:Class ;
              rdfs:label "Formation"@en ;
              rdfs:comment "The event of a group or organization coming into being."@en ;
              rdfs:subClassOf bio:IndividualEvent ;
              rdfs:isDefinedBy <http://purl.org/vocab/bio/0.1/> ;
              status:term_status "unstable" ;
              dct:issued "2011-06-10" .

bio:Disbanding rdf:type owl:Class ;
               rdfs:label "Disbanding"@en ;
               rdfs:comment "The event of a group or organization being disbanded."@en ;
               rdfs:subClassOf bio:IndividualEvent ;
               rdfs:isDefinedBy <http://purl.org/vocab/bio/0.1/> ;
               status:term_status "unstable" ;
               dct:issued "2011-06-10" .

bio:Performance rdf:type owl:Class ;
                rdfs:label "Performance"@en ;
                rdfs:comment "The event of an individual or a group of performers performing. Examples include concerts, plays, recitals, recordings, busking etc."@en ;
                rdfs:subClassOf bio:GroupEvent ;
                owl:equivalentClass mo:Performance ;
                rdfs:isDefinedBy <http://purl.org/vocab/bio/0.1/> ;
                status:term_status "unstable" ;
                dct:issued "2011-06-12" .

bio:Interval rdf:type owl:Class ;
             rdfs:label "Interval"@en ;
             rdfs:comment "A extended interval of time related to a particular state of affairs, such as the lifespan of a person or a period of employment."@en ;
             rdfs:isDefinedBy <http://purl.org/vocab/bio/0.1/> ;
             rdfs:subClassOf ns4:ProperInterval ;
             status:term_status "unstable" ;
             dct:issued "2010-05-03" .

bio:Relationship rdf:type owl:Class ;
                 rdfs:label "Agent Relationship"@en ;
                 rdfs:comment "A particular type of connection existing between people, groups or organizations related to or having dealings with each other."@en ;
                 rdfs:isDefinedBy <http://purl.org/vocab/bio/0.1/> ;
                 owl:equivalentClass rel:Relationship ;
                 status:term_status "unstable" ;
                 dct:issued "2011-06-14" .

bio:olb rdf:type rdf:Property ,
                 owl:DatatypeProperty ;
        rdfs:label "One-line bio"@en ;
        rdfs:comment "A one-line biography of the person."@en ;
        rdfs:domain foaf:Person ;
        rdfs:range rdfs:Literal ;
        rdfs:isDefinedBy <http://purl.org/vocab/bio/0.1/> ;
        skos:historyNote _:mor544133839145d ;
        status:term_status "stable" ;
        skos:changeNote _:mor54413383914be .

_:mor544133839145d rdf:value "Declared that this is a datatype property" ;
                   dct:date "2010-05-03" ;
                   dct:creator "Ian Davis" .

_:mor54413383914be rdf:value "Marked as a stable term" ;
                   dct:date "2010-05-04" ;
                   dct:creator "Ian Davis" .

bio:keywords rdf:type rdf:Property ,
                      owl:DatatypeProperty ;
             rdfs:label "Key Words"@en ;
             rdfs:comment "A comma delimited list of key words that describe a person."@en ;
             rdfs:domain foaf:Person ;
             rdfs:range rdfs:Literal ;
             rdfs:isDefinedBy <http://purl.org/vocab/bio/0.1/> ;
             rdfs:subPropertyOf dc:subject ;
             dct:issued "2003-07-28" ;
             skos:historyNote _:mor544133839153c ;
             status:term_status "stable" ;
             skos:changeNote _:mor544133839159c .

_:mor544133839153c rdf:value "Declared that this is a datatype property" ;
                   dct:date "2010-05-03" ;
                   dct:creator "Ian Davis" .

_:mor544133839159c rdf:value "Marked as a stable term" ;
                   dct:date "2010-05-04" ;
                   dct:creator "Ian Davis" .

bio:biography rdf:type rdf:Property ;
              rdfs:label "Biography"@en ;
              rdfs:comment "An extended description or account of someone's life."@en ;
              rdfs:domain foaf:Person ;
              rdfs:isDefinedBy <http://purl.org/vocab/bio/0.1/> ;
              status:term_status "unstable" ;
              dct:issued "2010-06-05" ;
              vann:usageNote "<p>It is expected that the value of this property is either a literal formatted with HTML markup or a pointer to an HTML document.</p>"^^rdf:XMLLiteral .

bio:date rdf:type rdf:Property ;
         rdfs:label "Date"@en ;
         label:plural "Dates"@en ;
         rdfs:comment "The date at which an event occurred."@en ;
         rdfs:domain bio:Event ;
         rdfs:subPropertyOf dc:date ;
         rdfs:isDefinedBy <http://purl.org/vocab/bio/0.1/> ;
         vann:usageNote '''<p>The date should be formatted as specified in <a href="http://www.w3.org/TR/NOTE-datetime">ISO8601</a>.
    For example: 2003-03-15 corresponds to the 15th March 2003, and 2003-03-15T13:21-05:00 corresponds to 15th March 2003, 8:21 am, US Eastern Standard Time.</p>'''^^rdf:XMLLiteral ;
         skos:changeNote _:mor5441338391634 ,
                         _:mor5441338391695 ;
         status:term_status "stable" .

_:mor5441338391634 rdf:value "Added a plural label" ;
                   dct:date "2010-05-03" ;
                   dct:creator "Ian Davis" .

_:mor5441338391695 rdf:value "Marked as a stable term" ;
                   dct:date "2010-05-04" ;
                   dct:creator "Ian Davis" .

bio:place rdf:type rdf:Property ;
          rdfs:label "Place"@en ;
          label:plural "Places"@en ;
          rdfs:comment "The place at which an event occurred."@en ;
          rdfs:domain bio:Event ;
          rdfs:isDefinedBy <http://purl.org/vocab/bio/0.1/> ;
          skos:changeNote _:mor5441338391717 ,
                          _:mor544133839177a ;
          status:term_status "stable" .

_:mor5441338391717 rdf:value "Added a plural label" ;
                   dct:date "2010-05-03" ;
                   dct:creator "Ian Davis" .

_:mor544133839177a rdf:value "Marked as a stable term" ;
                   dct:date "2010-05-04" ;
                   dct:creator "Ian Davis" .

bio:position rdf:type rdf:Property ,
                      owl:ObjectProperty ;
             rdfs:label "Position"@en ;
             label:plural "Positions"@en ;
             rdfs:comment "The employment position or public office involved in an event."@en ;
             rdfs:domain bio:Event ;
             rdfs:range foaf:Person ;
             rdfs:isDefinedBy <http://purl.org/vocab/bio/0.1/> ;
             rdfs:subPropertyOf bio:agent ;
             status:term_status "unstable" ;
             dct:issued "2010-05-05" .

bio:eventInterval rdf:type rdf:Property ,
                           owl:ObjectProperty ;
                  rdfs:label "Event Interval"@en ;
                  rdfs:comment "The interval during which the event occurs. This interval represents the exact interval of occurence for an event, it starts at the moment the event commences and finishes when the event concludes. In other words both the event and the interval start at the same instant of time and extend for the same duration."@en ;
                  rdfs:domain bio:Event ;
                  rdfs:range bio:Interval ;
                  rdfs:isDefinedBy <http://purl.org/vocab/bio/0.1/> ;
                  status:term_status "unstable" ;
                  dct:issued "2010-06-05" .

bio:father rdf:type rdf:Property ,
                    owl:ObjectProperty ,
                    owl:FunctionalProperty ;
           rdfs:label "Father"@en ;
           rdfs:comment "The biological father of a person, also known as the genitor."@en ;
           vann:usageNote 'Note that this is a strict definition of father that does not include non-biological relationships. The <a href="http://purl.org/vocab/relationship">Relationship</a> vocabulary may be more suitable for broader types of parent/child relation.'^^rdf:XMLLiteral ;
           rdfs:domain foaf:Person ;
           rdfs:range foaf:Person ;
           rdfs:isDefinedBy <http://purl.org/vocab/bio/0.1/> ;
           rdfs:subPropertyOf owl:differentFrom ,
                              rel:childOf ;
           skos:historyNote _:mor5441338391833 ;
           status:term_status "unstable" ;
           dct:issued "2010-05-03" .

_:mor5441338391833 rdf:value "Made subproperty of rel:childOf on suggestion of Gautier Poupeau" ;
                   dct:date "2010-06-06" ;
                   dct:creator "Ian Davis" .

bio:mother rdf:type rdf:Property ,
                    owl:ObjectProperty ,
                    owl:FunctionalProperty ;
           rdfs:label "Mother"@en ;
           rdfs:comment "The biological mother of a person, also known as the genetrix."@en ;
           vann:usageNote 'Note that this is a strict definition of mother that does not include non-biological relationships. The <a href="http://purl.org/vocab/relationship">Relationship</a> vocabulary may be more suitable for broader types of parent/child relation.'^^rdf:XMLLiteral ;
           rdfs:domain foaf:Person ;
           rdfs:range foaf:Person ;
           rdfs:isDefinedBy <http://purl.org/vocab/bio/0.1/> ;
           rdfs:subPropertyOf owl:differentFrom ,
                              rel:childOf ;
           skos:historyNote _:mor54413383918c2 ;
           status:term_status "unstable" ;
           dct:issued "2010-05-03" .

_:mor54413383918c2 rdf:value "Made subproperty of rel:childOf on suggestion of Gautier Poupeau" ;
                   dct:date "2010-06-06" ;
                   dct:creator "Ian Davis" .

bio:child rdf:type rdf:Property ,
                   owl:ObjectProperty ;
          rdfs:label "Child"@en ;
          label:plural "Children"@en ;
          rdfs:comment "A biological child of a person. "@en ;
          vann:usageNote 'Note that this is a strict definition of child that does not include adopted children, step-children or similar non-biological relationships. The <a href="http://purl.org/vocab/relationship">Relationship</a> vocabulary may be more suitable for broader types of parent/child relation.'^^rdf:XMLLiteral ;
          rdfs:domain foaf:Person ;
          rdfs:range foaf:Person ;
          rdfs:isDefinedBy <http://purl.org/vocab/bio/0.1/> ;
          rdfs:subPropertyOf owl:differentFrom ;
          owl:equivalentProperty rel:parentOf ;
          status:term_status "unstable" ;
          dct:issued "2010-05-03" ;
          skos:historyNote _:mor5441338391955 .

_:mor5441338391955 rdf:value "Made equivalent to rel:parentOf on suggestion of Gautier Poupeau" ;
                   dct:date "2010-06-06" ;
                   dct:creator "Ian Davis" .

bio:precedingEvent rdf:type rdf:Property ,
                            owl:ObjectProperty ,
                            owl:TransitiveProperty ;
                   rdfs:label "Preceding Event"@en ;
                   label:plural "Preceding Events"@en ;
                   rdfs:comment "An event that occurs and concludes at some time before this event."@en ;
                   rdfs:domain bio:Event ;
                   rdfs:range bio:Event ;
                   rdfs:isDefinedBy <http://purl.org/vocab/bio/0.1/> ;
                   rdfs:subPropertyOf owl:differentFrom ;
                   dct:issued "2010-05-06" .

bio:immediatelyPrecedingEvent rdf:type rdf:Property ,
                                       owl:ObjectProperty ;
                              rdfs:label "Immediately Preceding Event"@en ;
                              label:plural "Immediately Preceding Events"@en ;
                              rdfs:comment "An event that occurs and concludes immediately before this event."@en ;
                              rdfs:domain bio:Event ;
                              rdfs:range bio:Event ;
                              rdfs:isDefinedBy <http://purl.org/vocab/bio/0.1/> ;
                              rdfs:subPropertyOf owl:differentFrom ,
                                                 bio:precedingEvent ;
                              dct:issued "2010-05-06" .

bio:followingEvent rdf:type rdf:Property ,
                            owl:ObjectProperty ,
                            owl:TransitiveProperty ;
                   rdfs:label "Following Event"@en ;
                   label:plural "Following Events"@en ;
                   rdfs:comment "An event that starts at some time after this event."@en ;
                   rdfs:domain bio:Event ;
                   rdfs:range bio:Event ;
                   rdfs:isDefinedBy <http://purl.org/vocab/bio/0.1/> ;
                   rdfs:subPropertyOf owl:differentFrom ;
                   dct:issued "2010-05-06" .

bio:immediatelyFollowingEvent rdf:type rdf:Property ,
                                       owl:ObjectProperty ;
                              rdfs:label "Immediately Following Event"@en ;
                              label:plural "Immediately Following Events"@en ;
                              rdfs:comment "An event that starts immediately after this event."@en ;
                              rdfs:domain bio:Event ;
                              rdfs:range bio:Event ;
                              rdfs:isDefinedBy <http://purl.org/vocab/bio/0.1/> ;
                              rdfs:subPropertyOf owl:differentFrom ,
                                                 bio:followingEvent ;
                              dct:issued "2010-05-06" .

bio:concurrentEvent rdf:type rdf:Property ,
                             owl:ObjectProperty ,
                             owl:SymmetricProperty ;
                    rdfs:label "Concurrent Event"@en ;
                    label:plural "Concurrent Events"@en ;
                    rdfs:comment "An event that occurs while this event is occurring. The events need not start or conclude at the same times."@en ;
                    rdfs:domain bio:Event ;
                    rdfs:range bio:Event ;
                    rdfs:isDefinedBy <http://purl.org/vocab/bio/0.1/> ;
                    rdfs:subPropertyOf owl:differentFrom ;
                    dct:issued "2010-05-06" .

bio:initiatingEvent rdf:type rdf:Property ,
                             owl:ObjectProperty ;
                    rdfs:label "Initiating Event"@en ;
                    label:plural "Initiating Event"@en ;
                    rdfs:comment "An event that marks the start of an interval and/or relationship. The event contributes to and/or causes of the state of affairs that hold during the interval. For example a period of study may be initiated by an Enrolment event."@en ;
                    rdfs:range bio:Event ;
                    rdfs:isDefinedBy <http://purl.org/vocab/bio/0.1/> ;
                    rdfs:subPropertyOf owl:differentFrom ;
                    dct:issued "2010-05-06" .

bio:concludingEvent rdf:type rdf:Property ,
                             owl:ObjectProperty ;
                    rdfs:label "Concluding Event"@en ;
                    label:plural "Concluding Event"@en ;
                    rdfs:comment "An event that marks the end of an interval and/or relationship. The event changes of the state of affairs that held during the interval. For example a period of study may be concluded by a Graduation event."@en ;
                    rdfs:range bio:Event ;
                    rdfs:isDefinedBy <http://purl.org/vocab/bio/0.1/> ;
                    rdfs:subPropertyOf owl:differentFrom ;
                    dct:issued "2010-05-06" .

bio:agent rdf:type rdf:Property ,
                   owl:ObjectProperty ;
          rdfs:label "Agent"@en ;
          label:plural "Agents"@en ;
          rdfs:comment "A person, organization or group that plays a role in an event."@en ;
          rdfs:domain bio:Event ;
          rdfs:range foaf:Agent ;
          rdfs:isDefinedBy <http://purl.org/vocab/bio/0.1/> ;
          rdfs:subPropertyOf owl:differentFrom ;
          owl:inverseOf bio:event ;
          dct:issued "2010-05-05" .

bio:employer rdf:type rdf:Property ,
                      owl:ObjectProperty ;
             rdfs:label "Employer"@en ;
             label:plural "Employers"@en ;
             rdfs:comment "An agent that is involved in an event as an employer."@en ;
             rdfs:domain bio:Event ;
             rdfs:range foaf:Agent ;
             rdfs:isDefinedBy <http://purl.org/vocab/bio/0.1/> ;
             rdfs:subPropertyOf bio:agent ;
             dct:issued "2010-05-05" .

bio:state rdf:type rdf:Property ,
                   owl:ObjectProperty ;
          rdfs:label "State"@en ;
          label:plural "States"@en ;
          rdfs:comment "A country or independent territory that is involved in an event."@en ;
          rdfs:domain bio:Event ;
          rdfs:isDefinedBy <http://purl.org/vocab/bio/0.1/> ;
          rdfs:subPropertyOf bio:agent ;
          dct:issued "2010-05-05" .

bio:parent rdf:type rdf:Property ,
                    owl:ObjectProperty ;
           rdfs:label "Parent"@en ;
           label:plural "Parents"@en ;
           rdfs:comment "A person that takes the parent role in an event."@en ;
           rdfs:domain bio:Event ;
           rdfs:range foaf:Person ;
           rdfs:isDefinedBy <http://purl.org/vocab/bio/0.1/> ;
           rdfs:subPropertyOf bio:agent ;
           dct:issued "2010-05-05" .

bio:principal rdf:type rdf:Property ,
                       owl:ObjectProperty ;
              rdfs:label "Principal"@en ;
              label:plural "Principals"@en ;
              rdfs:comment "A person that takes the primary and most important role in an event. For example the principal in a Birth event would be the child being born and the principal in a Burial event would be the deceased person."@en ;
              rdfs:domain bio:Event ;
              rdfs:range foaf:Person ;
              rdfs:isDefinedBy <http://purl.org/vocab/bio/0.1/> ;
              rdfs:subPropertyOf bio:agent ;
              dct:issued "2010-05-05" .

bio:partner rdf:type rdf:Property ,
                     owl:ObjectProperty ;
            rdfs:label "Partner"@en ;
            label:plural "Partners"@en ;
            rdfs:comment "A person that is involved in a event as a partner in a relationship."@en ;
            rdfs:domain bio:Event ;
            rdfs:range foaf:Person ;
            rdfs:isDefinedBy <http://purl.org/vocab/bio/0.1/> ;
            rdfs:subPropertyOf bio:agent ;
            dct:issued "2010-05-05" .

bio:officiator rdf:type rdf:Property ,
                        owl:ObjectProperty ;
               rdfs:label "Officiator"@en ;
               label:plural "Officiators"@en ;
               rdfs:comment "A person that officiates at a ceremonial event."@en ;
               rdfs:domain bio:Event ;
               rdfs:range foaf:Person ;
               rdfs:isDefinedBy <http://purl.org/vocab/bio/0.1/> ;
               rdfs:subPropertyOf bio:agent ;
               dct:issued "2010-05-05" .

bio:witness rdf:type rdf:Property ,
                     owl:ObjectProperty ;
            rdfs:label "Witness"@en ;
            label:plural "Witnesses"@en ;
            rdfs:comment "A person that witnesses and can bear testimony to the occurrence of an event."@en ;
            rdfs:domain bio:Event ;
            rdfs:range foaf:Person ;
            rdfs:isDefinedBy <http://purl.org/vocab/bio/0.1/> ;
            rdfs:subPropertyOf bio:spectator ;
            dct:issued "2010-05-05" .

bio:spectator rdf:type rdf:Property ,
                       owl:ObjectProperty ;
              rdfs:label "Spectator"@en ;
              label:plural "Spectators"@en ;
              rdfs:comment "A person that is present at and observes the occurrence of at least part of an event."@en ;
              rdfs:domain bio:Event ;
              rdfs:range foaf:Person ;
              rdfs:isDefinedBy <http://purl.org/vocab/bio/0.1/> ;
              rdfs:subPropertyOf bio:agent ;
              dct:issued "2010-05-05" .

bio:organization rdf:type rdf:Property ,
                          owl:ObjectProperty ;
                 rdfs:label "Organization"@en ;
                 label:plural "Organizations"@en ;
                 rdfs:comment "An organization that plays a role in an event."@en ;
                 rdfs:domain bio:Event ;
                 rdfs:range foaf:Person ;
                 rdfs:isDefinedBy <http://purl.org/vocab/bio/0.1/> ;
                 rdfs:subPropertyOf bio:agent ;
                 dct:issued "2010-05-05" .

bio:event rdf:type rdf:Property ,
                   owl:ObjectProperty ;
          rdfs:label "Life Event"@en ;
          label:plural "Life Events"@en ;
          rdfs:comment "An event associated with a person, group or organization."@en ;
          rdfs:domain foaf:Agent ;
          rdfs:range bio:Event ;
          rdfs:isDefinedBy <http://purl.org/vocab/bio/0.1/> ;
          rdfs:subPropertyOf owl:differentFrom ;
          skos:historyNote _:mor5441338391b6c ,
                           _:mor5441338391bc8 ;
          skos:changeNote _:mor5441338391c22 ;
          owl:inverseOf bio:agent .

_:mor5441338391b6c rdf:value "Made a subproperty of owl:differentFrom" ;
                   dct:date "2010-05-03" ;
                   dct:creator "Ian Davis" .

_:mor5441338391bc8 rdf:value "Changed domain to foaf:Agent" ;
                   dct:date "2011-06-14" ;
                   dct:creator "Ian Davis" .

_:mor5441338391c22 rdf:value "Added a plural label" ;
                   dct:date "2010-05-03" ;
                   dct:creator "Ian Davis" .

bio:birth rdf:type rdf:Property ,
                   owl:ObjectProperty ;
          rdfs:subPropertyOf bio:event ,
                             owl:differentFrom ;
          rdfs:label "Birth Event"@en ;
          label:plural "Birth Events"@en ;
          rdfs:comment "An birth event associated with a person, group or organization."@en ;
          rdfs:domain foaf:Agent ;
          rdfs:range bio:Birth ;
          rdfs:isDefinedBy <http://purl.org/vocab/bio/0.1/> ;
          skos:historyNote _:mor5441338391cb3 .

_:mor5441338391cb3 rdf:value "Proposed addition of the property" ;
                   dct:date "2011-07-12" ;
                   dct:creator "Alexandre Passant" .

bio:death rdf:type rdf:Property ,
                   owl:ObjectProperty ;
          rdfs:subPropertyOf bio:event ,
                             owl:differentFrom ;
          rdfs:label "Death Event"@en ;
          label:plural "Death Events"@en ;
          rdfs:comment "An death event associated with a person, group or organization."@en ;
          rdfs:domain foaf:Agent ;
          rdfs:range bio:Death ;
          rdfs:isDefinedBy <http://purl.org/vocab/bio/0.1/> ;
          skos:historyNote _:mor5441338391d3b .

_:mor5441338391d3b rdf:value "Proposed addition of the property" ;
                   dct:date "2011-07-12" ;
                   dct:creator "Alexandre Passant" .

bio:participant rdf:type rdf:Property ,
                         owl:ObjectProperty ;
                rdfs:label "Participant"@en ;
                label:plural "Participants"@en ;
                rdfs:comment "A person, group or organization that participates in a relationship for some time."@en ;
                rdfs:domain bio:Relationship ;
                rdfs:range foaf:Agent ;
                rdfs:isDefinedBy <http://purl.org/vocab/bio/0.1/> ;
                rdfs:subPropertyOf owl:differentFrom ;
                owl:equivalentProperty rel:participant ;
                owl:inverseOf bio:relationship ;
                dct:issued "2011-06-14" .

bio:relationship rdf:type rdf:Property ,
                          owl:ObjectProperty ;
                 rdfs:label "Relationship"@en ;
                 label:plural "Relationships"@en ;
                 rdfs:comment "A relationship that a person, group or organization participates in for some time."@en ;
                 rdfs:domain foaf:Agent ;
                 rdfs:range bio:Relationship ;
                 rdfs:isDefinedBy <http://purl.org/vocab/bio/0.1/> ;
                 rdfs:subPropertyOf owl:differentFrom ;
                 owl:equivalentProperty rel:participantIn ;
                 owl:inverseOf bio:participant ;
                 dct:issued "2011-06-14" .

bio:interval rdf:type rdf:Property ,
                      owl:ObjectProperty ;
             rdfs:label "Relationship Interval"@en ;
             rdfs:comment "The interval during which the relationship persists."@en ;
             rdfs:domain bio:Relationship ;
             rdfs:range bio:Interval ;
             rdfs:isDefinedBy <http://purl.org/vocab/bio/0.1/> ;
             status:term_status "unstable" ;
             dct:issued "2010-06-05" .

bio:termgroup1 rdf:type rdf:Bag ;
               rdfs:label "Properties of a person"@en ;
               rdf:_1 bio:olb ;
               rdf:_2 bio:biography ;
               rdf:_3 bio:keywords ;
               rdf:_4 bio:father ;
               rdf:_5 bio:mother ;
               rdf:_6 bio:child ;
               rdf:_7 bio:event ;
               rdf:_8 bio:birth ;
               rdf:_9 bio:death .

bio:termgroup2 rdf:type rdf:Bag ;
               rdfs:label "Types of event"@en ;
               rdf:_1 bio:Event ;
               rdf:_2 bio:IndividualEvent ;
               rdf:_3 bio:GroupEvent ;
               rdf:_4 bio:Accession ;
               rdf:_5 bio:Adoption ;
               rdf:_6 bio:Annulment ;
               rdf:_7 bio:Assassination ;
               rdf:_8 bio:Baptism ;
               rdf:_9 bio:BarMitzvah ;
               rdf:_10 bio:BasMitzvah ;
               rdf:_11 bio:Birth ;
               rdf:_12 bio:Burial ;
               rdf:_13 bio:PositionChange ;
               rdf:_14 bio:Coronation ;
               rdf:_15 bio:Cremation ;
               rdf:_16 bio:Death ;
               rdf:_17 bio:Demotion ;
               rdf:_18 bio:Dismissal ;
               rdf:_19 bio:Divorce ;
               rdf:_20 bio:Emigration ;
               rdf:_21 bio:Employment ;
               rdf:_22 bio:Execution ;
               rdf:_23 bio:Enrolment ;
               rdf:_24 bio:Funeral ;
               rdf:_25 bio:Graduation ;
               rdf:_26 bio:Imprisonment ;
               rdf:_27 bio:Inauguration ;
               rdf:_28 bio:Investiture ;
               rdf:_29 bio:Marriage ;
               rdf:_30 bio:Murder ;
               rdf:_31 bio:NameChange ;
               rdf:_32 bio:Naturalization ;
               rdf:_33 bio:Ordination ;
               rdf:_34 bio:Promotion ;
               rdf:_35 bio:Redundancy ;
               rdf:_36 bio:Resignation ;
               rdf:_37 bio:Retirement .

bio:termgroup3 rdf:type rdf:Bag ;
               rdfs:label "Properties of an event"@en ;
               rdf:_1 bio:date ;
               rdf:_2 bio:place ;
               rdf:_3 bio:state ;
               rdf:_4 bio:position .

bio:termgroup4 rdf:type rdf:Bag ;
               rdfs:label "Properties that relate an event to an agent"@en ;
               rdf:_1 bio:agent ;
               rdf:_2 bio:parent ;
               rdf:_3 bio:employer ;
               rdf:_4 bio:officiator ;
               rdf:_5 bio:organization ;
               rdf:_6 bio:principal ;
               rdf:_7 bio:partner ;
               rdf:_8 bio:witness ;
               rdf:_9 bio:spectator .

bio:termgroup5 rdf:type rdf:Bag ;
               rdfs:label "Properties that relate an event to another event"@en ;
               rdf:_1 bio:concurrentEvent ;
               rdf:_2 bio:followingEvent ;
               rdf:_3 bio:precedingEvent ;
               rdf:_4 bio:immediatelyFollowingEvent ;
               rdf:_5 bio:immediatelyPrecedingEvent .

<http://purl.org/vocab/bio/examples/1> rdf:type ov:SchemaExample ;
                                       rdfs:label "A Biography of Henry VIII, King of England" ;
                                       rdfs:comment """<p>Based on information at <a href="http://en.wikipedia.org/wiki/Henry_VIII_of_England">Wikipedia</a> and <a href="http://www3.dcs.hull.ac.uk/cgi-bin/gedlkup/n=royal?royal00828">Hull University</a></p>
<pre><code>@prefix bio: &lt;http://purl.org/vocab/bio/0.1/&gt; .
@prefix foaf: &lt;http://xmlns.com/foaf/0.1/&gt; .
@prefix rdfs: &lt;http://www.w3.org/2000/01/rdf-schema#&gt; .

_:henryviii
  a foaf:Person
  ; foaf:name "Henry VIII, King of England"
  ; bio:father _:henryvii
  ; bio:mother _:elizplantagenet
  ; bio:child _:child1, _:child2, _:child3, _:child4, _:child5, _:child6, _:child7, _:child8
  ; bio:birth _:birth
  ; bio:death _:death
  ; bio:event _:burial, _:accession, _:coronation, _:marriage1
            , _:marriage2, _:marriage3, _:marriage4, _:marriage5, _:marriage6
  .

_:henryvii
  a foaf:Person
  ; foaf:name "Henry VII Tudor, King of England"
  ; bio:child _:henryviii
  .

_:elizplantagenet
  a foaf:Person
  ; foaf:name "Elizabeth of York"
  ; bio:child _:henryviii
  .
  
_:birth
  a bio:Birth
  ; rdfs:label "The birth of Henry VIII to Henry VII and Elizabeth Plantagenet on 28 June 1491"
  ; bio:date "1491-06-28"
  ; bio:place &lt;http://dbpedia.org/resource/Palace_of_Placentia&gt;
  ; bio:parent _:henryvii, _:elizplantagenet
  ; bio:principal _:henryviii
  .

_:death
  a bio:Death
  ; rdfs:label "The death of Henry VIII on 28 January 1547"
  ; bio:date "1547-01-28"
  ; bio:place &lt;http://dbpedia.org/resource/Palace_of_Whitehall&gt;
  ; bio:principal _:henryviii
  .
  

_:accession
  a bio:Accession
  ; rdfs:label "The accession of Henry VIII to the throne of England on 21 April 1509"
  ; bio:date "1509-06-24"
  ; bio:principal _:henryviii
  ; bio:state &lt;http://dbpedia.org/resource/Kingdom_of_England&gt;
  ; bio:immediatelyPrecedingEvent [ a bio:Death
                                    ; rdfs:label "The death of Henry VII on 9 May 1509"
                                    ; bio:date "1509-05-09"
                                    ; bio:place &lt;http://dbpedia.org/resource/Richmond_Palace&gt;
                                    ; bio:principal _:henryvii
                                  ]
  .

_:coronation
  a bio:Coronation
  ; rdfs:label "The coronation of Henry VIII as King of England on 24 June 1509"
  ; bio:date "1509-06-24"
  ; bio:place &lt;http://dbpedia.org/page/Westminster_Abbey&gt;
  ; bio:principal _:henryviii
  ; bio:precedingEvent _:accession
  .

_:burial
  a bio:Burial
  ; rdfs:label "The burial of Henry VII at St.George's Chapel, Windsor Castle,England"
  ; bio:place &lt;http://dbpedia.org/resource/St_George%E2%80%99s_Chapel%2C_Windsor&gt;
  ; bio:principal _:henryviii
  ; bio:precedingEvent _:death
  .

_:marriage1
  a bio:Marriage
  ; rdfs:label "The marriage of Henry VIII and Catherine of Aragon"
  ; bio:date "1509-06-11"
  ; bio:place &lt;http://dbpedia.org/resource/Palace_of_Placentia&gt;
  ; bio:partner _:henryvii, _:catharagon
  .

_:annulment1
  a bio:Annulment
  ; rdfs:label "The annulment of the marriage between Henry VIII and Catherine of Aragon"
  ; bio:date "1533-05-23"
  ; bio:partner _:henryvii, _:catharagon 
  ; bio:officiator &lt;http://dbpedia.org/resource/Thomas_Cranmer&gt;
  .

_:catharagon
  a foaf:Person
  ; foaf:name "Anne Boleyn"
  ; bio:child _:child1, _:child2, _:child3, _:child4, _:child5
  ; bio:event _:marriage1, _:annulment1
  .

_:child1
  a foaf:Person
  ; rdfs:label "Unnamed daughter of Henry VIII and Catherine of Aragon"
  ; bio:event [ a bio:Birth
                ; bio:date "1510-01-31"
                ; bio:principal _:child1
                ; bio:parent _:henryviii, _:catharagon
              ]
  ; bio:event [ a bio:Death
                ; bio:date "1510-02-02"
                ; bio:principal _:child1
              ]
  .

_:child2
  a foaf:Person
  ; foaf:name "Henry"
  ; bio:event [ a bio:Birth
                ; bio:date "1511-01-01"
                ; bio:principal _:child2
                ; bio:parent _:henryviii, _:catharagon
              ]
  ; bio:event [ a bio:Death
                ; bio:date "1511-02-22"
                ; bio:principal _:child2
              ]
  .
  
_:child3
  a foaf:Person
  ; foaf:name "Henry"
  ; bio:event [ a bio:Birth
                ; bio:date "1514-12"
                ; bio:principal _:child3
                ; bio:parent _:henryviii, _:catharagon
              ]
  ; bio:event [ a bio:Death
                ; bio:principal _:child3
              ]
  .

_:child4
  a foaf:Person
  ; foaf:name "Mary"
  ; bio:event [ a bio:Birth
                ; bio:date "1516-02-18"
                ; bio:principal _:child4
                ; bio:parent _:henryviii, _:catharagon
              ]
  ; bio:event [ a bio:Death
                ; bio:date "1558-11-17"
                ; bio:principal _:child4
              ]
  .


_:child5
  a foaf:Person
  ; rdfs:label "Unnamed daughter of Henry VIII and Catherine of Aragon"
  ; bio:event [ a bio:Birth
                ; bio:date "1518-11"
                ; bio:principal _:child5
                ; bio:parent _:henryviii, _:catharagon
              ]
  ; bio:event [ a bio:Death
                ; bio:principal _:child5
              ]
  .
  

_:marriage2
  a bio:Marriage
  ; rdfs:label "The marriage of Henry VIII and Anne Boleyn"
  ; bio:date "1533-01-25"
  ; bio:partner _:henryvii, _:anneboleyn
  ; bio:place &lt;http://dbpedia.org/resource/Westminster_Abbey&gt;
  .

_:anneboleyn
  a foaf:Person
  ; foaf:name "Anne Boleyn"
  ; bio:child _:child6
  ; bio:event _:marriage2, _:annulment2, _:anneboleyn-death
  .

_:annulment2
  a bio:Annulment
  ; rdfs:label "The annulment of the marriage between Henry VIII and Anne Boleyn"
  ; bio:date "1536-05-17"
  ; bio:partner _:henryvii, _:anneboleyn 
  .
  
_:anneboleyn-death
  a bio:Execution
  ; rdfs:label "The beheading of Anne Boleyn"
  ; bio:date "1536-05-19"
  ; bio:place &lt;http://dbpedia.org/resource/Tower_of_London&gt;
  ; bio:principal _:anneboleyn
  .

_:child6
  a foaf:Person
  ; foaf:name "Elizabeth"
  ; bio:event [ a bio:Birth
                ; bio:date "1533-09-07"
                ; bio:principal _:child6
                ; bio:parent _:henryviii, _:anneboleyn
              ]
  ; bio:event [ a bio:Death
                ; bio:date "1603-03-24"
                ; bio:principal _:child6
              ]
  .

_:marriage3
  a bio:Marriage
  ; bio:date "1536-05-20"
  ; bio:partner _:henryviii, _:janeseymour
  ; bio:place &lt;http://dbpedia.org/resource/York_Place&gt;
  .

_:janeseymour
  a foaf:Person
  ; foaf:name "Jane Seymour"
  ; bio:event _:marriage3, _:janeseymour-death
  ; bio:child _:child7
  .

_:janeseymour-death
  a bio:Death
  ; rdfs:label "The death of Jane Seymour on 24 October 1537"
  ; bio:date "1537-10-24"
  ; bio:principal _:janeseymour
  ; bio:place &lt;http://dbpedia.org/resource/Hampton_Court_Palace&gt;
  .
  

_:child7
  a foaf:Person
  ; foaf:name "Edward"
  ; bio:event [ a bio:Birth
                ; bio:date "1537-10-12"
                ; bio:principal _:child7
                ; bio:parent _:henryviii, _:janeseymour
                ; bio:place &lt;http://dbpedia.org/resource/Hampton_Court_Palace&gt;
              ]
  ; bio:event [ a bio:Accession
                ; bio:immediatelyPrecedingEvent _:death
              ]
  ; bio:event [ a bio:Death
                ; bio:date "1553-07-06"
                ; bio:principal _:child7
                ; bio:place &lt;http://dbpedia.org/resource/Palace_of_Placentia&gt;
              ]
  .

_:marriage4
  a bio:Marriage
  ; bio:date "1540-01-06"
  ; bio:partner _:henryvii, _:annecleves
  ; bio:place &lt;http://dbpedia.org/resource/Palace_of_Placentia&gt;
  ; bio:officiator &lt;http://dbpedia.org/resource/Thomas_Cranmer&gt;
  .
    
_:annulment3
  a bio:Annulment
  ; rdfs:label "The annulment of the marriage between Henry VIII and Anne of Cleves"
  ; bio:date "1540-07-09"
  ; bio:partner _:henryviii, _:annecleves
  .

_:annecleves
  a foaf:Person
  ; foaf:name "Anne of Cleves"
  ; bio:event _:marriage4, _:annulment3
  .

_:marriage5
  a bio:Marriage
  ; bio:date "1540-07-28"
  ; bio:partner _:henryviii, _:cathhoward
  ; bio:place &lt;http://dbpedia.org/resource/Oatlands_Palace&gt;
  .
  
_:cathhoward
  a foaf:Person
  ; foaf:name "Catherine Howard"
  ; bio:event _:marriage5, _:cathhoward-death
  .
  
_:cathhoward-death
  a bio:Execution
  ; rdfs:label "The beheading of Catherine Howard"
  ; bio:date "1542-02-13"
  ; bio:place &lt;http://dbpedia.org/resource/Tower_of_London&gt;
  ; bio:principal _:cathhoward
  .

_:marriage6
  a bio:Marriage
  ; rdfs:label "The marriage between Henry VIII and Catherine Parr"
  ; bio:date "1543-07-12"
  ; bio:place &lt;http://dbpedia.org/resource/Hampton_Court_Palace&gt;
  ; bio:partner _:henryviii, _:cathparr
  .
  
_:cathparr
  a foaf:Person
  ; foaf:name "Catherine Parr"
  ; bio:event _:marriage6
  .


_:elizblount
  a foaf:Person
  ; foaf:name "Elizabeth Blount"
  ; bio:child _:child8
  .
  
_:child8
  a foaf:Person
  ; foaf:name "Henry FitzRoy"
  ; foaf:mother _:elizblount
  ; foaf:father _:henryviii
  ; bio:event [ a bio:Birth
                ; bio:principal _:child8
                ; bio:date "1519-06-15"
                ; bio:parent _:henryviii, _:elizblount
                ; bio:place &lt;http://dbpedia.org/resource/Blackmore&gt;
                ]
  .

_:marriage1-interval
  a bio:Interval
  ; rdfs:label "The period of time during which Henry VIII and Catherine of Aragon were married"
  ; bio:initiatingEvent _:marriage1
  ; bio:concludingEvent _:annulment1
  .

_:marriage2-interval
  a bio:Interval
  ; rdfs:label "The period of time during which Henry VIII and Anne Boleyn were married"
  ; bio:initiatingEvent _:marriage2
  ; bio:concludingEvent _:annulment2
  .
  
_:marriage3-interval
  a bio:Interval
  ; rdfs:label "The period of time during which Henry VIII and Jane Seymour were married"
  ; bio:initiatingEvent _:marriage3
  ; bio:concludingEvent _:janeseymour-death
  .

_:marriage4-interval
  a bio:Interval
  ; rdfs:label "The period of time during which Henry VIII and Anne of Cleves were married"
  ; bio:initiatingEvent _:marriage4
  ; bio:concludingEvent _:annulment3
  .

_:marriage5-interval
  a bio:Interval
  ; rdfs:label "The period of time during which Henry VIII and Catherine Howard were married"
  ; bio:initiatingEvent _:marriage5
  ; bio:terminatingEvent _:cathhoward-death
  .

_:marriage6-interval
  a bio:Interval
  ; rdfs:label "The period of time during which Henry VIII and Catherine Parr were married"
  ; bio:initiatingEvent _:marriage6
  ; bio:terminatingEvent _:henryviii-death
  .
</code></pre>
"""^^rdf:XMLLiteral .